src/asn1/ASN1.Low.INTEGER.fst
@@ -1,0 +1,269 @@
+module ASN1.Low.INTEGER
+
+open ASN1.Base
+open ASN1.Spec.INTEGER
+open ASN1.Low.Base
+open LowParse.Bytes
+
+open FStar.Integers
+
+module HS = FStar.HyperStack
+module HST = FStar.HyperStack.ST
+module MB = LowStar.Monotonic.Buffer
+module B = LowStar.Buffer
+module Cast = FStar.Int.Cast
+module E = LowParse.Endianness
+module LE = LowParse.Low.Endianness
+
+let len_of_asn1_integer
+  (value: datatype_of_asn1_type INTEGER)
+: Tot (len: asn1_int32_of_type INTEGER { v len == length_of_asn1_integer value } )
+= if      0l         <= value && value <= 0x7Fl      then
+  ( 1ul )
+  else if 0x7Fl       < value && value <= 0xFFl       then
+  ( 2ul )
+  else if 0xFFl       < value && value <= 0x7FFFl     then
+  ( 2ul )
+  else if 0x7FFFl     < value && value <= 0xFFFFl     then
+  ( 3ul )
+  else if 0xFFFFl     < value && value <= 0x7FFFFFl   then
+  ( 3ul )
+  else if 0x7FFFFFl   < value && value <= 0xFFFFFFl   then
+  ( 4ul )
+  else if 0xFFFFFFl   < value && value <= 0x7FFFFFFFl then
+  ( 4ul )
+
+(*
+NOTE: Since there are no low-level machine-integer to bytes implementations
+      available, the (big-endian) serialization of integers are tricky. For
+      1-byte, 2-byte and 4-byte integers, we could use `LowStar.Endianness`
+      16-bit, 32-bit integer store interfaces. For 3-byte, we may need some
+      magic.
+*)
+
+open LowParse.Low.BoundedInt
+
+#restart-solver
+#push-options "--query_stats --z3rlimit 32"
+let serialize32_asn1_integer
+  (len: asn1_int32_of_type INTEGER)
+: Tot (serializer32 (serialize_asn1_integer (v len)))
+= fun (value: datatype_of_asn1_type INTEGER { v len == length_of_asn1_integer value })
+    (#rrel #rel: _)
+    (b: B.mbuffer byte_t rrel rel)
+    (pos: size_t)
+->(* 1-byte integer with the most-significant bit `0` *)
+  if      (0l         <= value && value <= 0x7Fl      ) then
+  ( admit (); (* Prf *) serialize_asn1_integer_unfold (length_of_asn1_integer value) value
+  ; let b0: byte = cast #(Signed W32) #(Unsigned W8) value in
+    (* Prf *) E.reveal_be_to_n (Seq.create 1 b0)
+  ; (* Prf *) E.reveal_be_to_n (Seq.slice (Seq.create 1 b0) 1 1)
+  ; mbuffer_upd
+    (* dst *) (b)
+    (*range*) (v pos) (v pos + 1)
+    (* pos *) (pos)
+    (* val *) (b0)
+  ; (*return*) 1ul )
+
+  (* 1-byte integer with the most-significant bit `1` *)
+  else if (0x7Fl       < value && value <= 0xFFl      ) then
+  ( admit ()
+  ; (* Prf *) serialize_asn1_integer_unfold (length_of_asn1_integer value) value;
+    (* Prf *) let h0 = HST.get () in
+    (* Prf *) writable_weaken
+              (* buf *) (b)
+              (*range*) (v pos) (v pos + 2)
+              (* mem *) (h0)
+              (* from*) (v pos)
+              (* to  *) (v pos + 1);
+    (* NOTE: Serializing the leading zero. *)
+    mbuffer_upd
+      (* dst *) (b)
+      (*range*) (v pos) (v pos + 1)
+      (* pos *) (pos)
+      (* val *) (0x00uy);
+    (* Prf *) let h1 = HST.get () in
+    (* Prf *) writable_modifies
+              (* buf *) (b)
+              (*range*) (v pos) (v pos + 2)
+              (* mem *) (h0)
+              (* loc *) (B.loc_none)
+              (* mem *) (h1);
+    (* Prf *) writable_weaken
+              (* buf *) (b)
+              (*range*) (v pos) (v pos + 2)
+              (* mem *) (h1)
+              (* from*) (v pos + 1)
+              (* to  *) (v pos + 2);
+    (* NOTE: Serializing the 1-byte integer. *)
+    let b0: byte = cast #(Signed W32) #(Unsigned W8) value in
+    (* Prf *) E.reveal_be_to_n (Seq.create 1 b0);
+    (* Prf *) E.reveal_be_to_n (Seq.slice (Seq.create 1 b0) 1 1);
+    mbuffer_upd
+      (* dst *) (b)
+      (*range*) (v pos) (v pos + 2)
+      (* pos *) (pos + 1ul)
+      (* val *) (b0);
+    (* Prf *) let h2 = HST.get () in
+    (* Prf *) Seq.lemma_split
+              (*slice*) (Seq.slice (B.as_seq h2 b) (v pos) (v pos + 2))
+              (* at  *) (1);
+    (* Prf *) B.modifies_buffer_from_to_elim
+              (* buf *) (b)
+              (*frame*) (pos) (pos + 1ul)
+              (* new *) (B.loc_buffer_from_to b (pos + 1ul) (pos + 2ul))
+              (* mem *) (h1) (h2);
+  (*return*) 2ul )
+
+  (* 2-byte integer with the most-significant bit `0` *)
+  else if (0xFFl       < value && value <= 0x7FFFl    ) then
+  ( (* Prf *) serialize_asn1_integer_unfold (length_of_asn1_integer value) value;
+    (* Prf *) let h0 = HST.get () in
+    (* Prf *) LE.writable_store_pre
+              (* buf *) b
+              (* from*) (v pos)
+              (* len *) 2
+              (*  p  *) (fun s -> E.be_to_n s == v #(Signed W32) value)
+              (* mem *) h0;
+    (* Prf *) let h1 = HST.get () in
+    LE.store16_be_i
+      (* buf *) b
+      (* pos *) pos
+      (* val *) (cast #(Signed W32) #(Unsigned W16) value);
+    (* Prf *) LE.store_post_modifies
+              (* buf *) b
+              (* from*) (v pos)
+              (* len *) 2
+              (*  p  *) (fun s -> E.be_to_n s == v #(Signed W32) value);
+  (*return*) 2ul )
+
+  (* 2-byte integer with the most-significant bit `1` *)
+  else if (0x7FFFl       < value && value <= 0xFFFFl    ) then
+  ( (* Prf *) serialize_asn1_integer_unfold (length_of_asn1_integer value) value;
+    (* Prf *) serialize_bounded_integer_spec 2 (cast #(Signed W32) #(Unsigned W32) value);
+    let h0 = HST.get () in
+    writable_weaken b (v pos) (v pos + 3) h0 (v pos) (v pos + 1);
+    mbuffer_upd b (v pos) (v pos + 3) pos 0x00uy;
+    let h1 = HST.get () in
+    writable_modifies b (v pos) (v pos + 3) h0 B.loc_none h1;
+    writable_weaken b (v pos) (v pos + 3) h1 (v pos + 1) (v pos + 3);
+    let offset = serialize32_bounded_integer_2 () (cast #(Signed W32) #(Unsigned W32) value) b pos in
+    let h2 = HST.get () in
+    B.modifies_buffer_from_to_elim b pos (pos + 1ul) (B.loc_buffer_from_to b (pos + 1ul) (pos + 3ul)) h1 h2;
+  (*return*) 1ul + offset )
+  else admit ()
+
+
+(*)
+  (* NOTE: 3-byte integer with the most-significant bit `0` *)
+  else if (0xFFFFl      < value && value <= 0x7FFFFFl  ) then
+  ( (* Prf *) serialize_asn1_integer_unfold (length_of_asn1_integer value) value;
+    (* Prf *) assert_norm (v #(Signed W32) value < pow2 (8 * 3 - 1) /\
+                           v #(Signed W32) value < pow2 (8 * 3));
+    (* Prf *) E.reveal_n_to_be 3 (v #(Signed W32) value);
+    (* NOTE: Serialize the first and second bytes of this 3-byte integer. *)
+    let v01: uint_16 = cast #(Signed W32) #(Unsigned W16) (value / 0x100l) in
+    (* Prf *) let h0 = HST.get () in
+    (* Prf *) writable_weaken
+              (* buf *) (b)
+              (*range*) (v pos) (v pos + 3)
+              (* mem *) (h0)
+              (* from*) (v pos)
+              (* to  *) (v pos + 2);
+    (* Prf *) LE.writable_store_pre
+              (* dst *) (b)
+              (* from*) (v pos)
+              (* len *) (2)
+              (*predi*) (fun s -> E.be_to_n s == v v01)
+              (* mem *) (h0);
+    LE.store16_be_i
+    (* dst *) (b)
+    (* pos *) (pos)
+    (* val *) (v01);
+    (* Prf *) let h1 = HST.get () in
+    (* Prf *) LE.store_post_modifies
+              (* dst *) (b)
+              (* from*) (v pos)
+              (* len *) (2)
+              (*predi*) (fun s -> E.be_to_n s == v v01)
+              (* mem *) (h0)
+              (* mem'*) (h1);
+    (* NOTE: Serialize the third byte of this 3-byte integer. *)
+    let b2: byte = cast #(Signed W32) #(Unsigned W8) (value % 0x100l) in
+    (* Prf *) let h2 = HST.get () in
+    (* Prf *) E.reveal_be_to_n (Seq.create 1 b2);
+    (* Prf *) E.reveal_be_to_n (Seq.slice (Seq.create 1 b2) 1 1);
+    (* Prf *) writable_modifies
+              (* buf *) (b)
+              (*range*) (v pos) (v pos + 3)
+              (* mem *) (h0)
+              (* loc *) (B.loc_none)
+              (* mem'*) (h1);
+    (* Prf *) writable_weaken
+              (* buf *) (b)
+              (*range*) (v pos) (v pos + 3)
+              (* mem *) (h1)
+              (* from*) (v pos + 2)
+              (* to  *) (v pos + 3);
+    mbuffer_upd
+    (* dst *) (b)
+    (*range*) (v pos) (v pos + 3)
+    (* pos *) (pos + 2ul)
+    (* val *) (b2);
+    (* Prf *) Seq.lemma_split
+              (*slice*) (Seq.slice (B.as_seq h2 b) (v pos) (v pos + 3))
+              (* at  *) (2);
+    (* Prf *) B.modifies_buffer_from_to_elim
+              (* buf *) (b)
+              (*frame*) (pos) (pos + 2ul)
+              (* new *) (B.loc_buffer_from_to b (pos + 2ul) (pos + 3ul))
+              (* mem *) (h1) (h2);
+  (*return*) 3ul )
+
+  else (admit ())
+
+(*)
+  (* 2-byte integer with the mort-significant bit `0` *)
+  else if (0xFFl       < value && value <= 0x7FFFl    ) then
+  ( admit ();
+    (* Prf *) serialize_asn1_integer_unfold (length_of_asn1_integer value) value
+  ; (* Prf *) serialize_bounded_integer_spec 2 (cast #(Signed W32) #(Unsigned W32) value)
+  ; let offset = serialize32_bounded_integer_2 ()
+    (* val *) (cast #(Signed W32) #(Unsigned W32) value)
+    (* dst *) (b)
+    (* pos *) (pos) in
+  (*return*) offset )
+  else
+  ( admit () )
+#pop-options
+
+
+  // if      (0l         <= value && value <= 0x7Fl      ) then
+  // ( (* Prf *) serialize_asn1_integer_unfold (length_of_asn1_integer value) value
+  // ; let b0: byte = cast #(Signed W32) #(Unsigned W8) value in
+  //   (* Prf *) E.reveal_be_to_n (Seq.create 1 b0)
+  // ; (* Prf *) E.reveal_be_to_n (Seq.slice (Seq.create 1 b0) 1 1)
+  // ; mbuffer_upd
+  //   (* dst *) (b)
+  //   (*range*) (v pos) (v pos + 1)
+  //   (* pos *) (pos)
+  //   (* val *) (b0)
+  // ; (*return*) 1ul )
+
+  // (* 3-byte integer with the most-significant bit `1` *)
+  // else if (0x7FFFFFl     < value && value <= 0xFFFFFFl    ) then
+  // ( (* Prf *) serialize_asn1_integer_unfold (length_of_asn1_integer value) value
+  // ; let b0: byte = cast #(Signed W32) #(Unsigned W8) (value / 0x10000l) in
+  //   let v12: uint_16 = cast #(Signed W32) #(Unsigned W16) (value % 0x10000l) in
+  //   (* Prf *) E.reveal_be_to_n (Seq.create 1 b0)
+  // ; (* Prf *) E.reveal_be_to_n (Seq.slice (Seq.create 1 b0) 1 1)
+  // ; mbuffer_upd
+  //   (* dst *) (b)
+  //   (*range*) (v pos) (v pos + 1)
+  //   (* pos *) (pos)
+  //   (* val *) (b0)
+  // ; LE.store16_be_i
+  //   (* dst *) (b)
+  //   (* pos *) (pos + 1ul)
+  //   (* val *) (v12)
+  // ; (*return*) 3ul)
